Add helper functions back since they introduce less SMT goals

rupicola/refinements2/CompilableWP.fst
@@ -40,21 +40,6 @@ type fs_oexp (g:env) (a:Type) (wpG:spec_env g a) =
   fsG:fs_env g -> PURE a (wpG fsG)
 
 unfold
-val wp_lambda : #g :env ->
-                #a :Type ->
-                #b :Type ->
-                wpBody:spec_env (extend a g) b ->
-                spec_env g (a -> b)
-
-let wp_lambda #g #a #b wpBody fsG : pure_wp (a -> b) =
-  reveal_opaque (`%pure_wp_monotonic) (pure_wp_monotonic);
-  fun (p:pure_post (a -> b)) ->
-    forall (f:a -> b).
-      (forall (p':pure_post b) (fsG':fs_env (extend a g)).
-        fsG == fs_tail fsG' ==>  wpBody fsG' p' ==>  p' (f (fs_hd fsG'))
-      ) ==>  p f
-
-unfold
 val helper_var0 : g:env ->
                  a:Type ->
                  fs_oexp (extend a g) a (fun fsG -> ret (fs_hd fsG))
@@ -76,25 +61,116 @@ val helper_var2 : g:env ->
                   fs_oexp (extend c (extend b (extend a g))) a (fun fsG -> ret (fs_hd (fs_tail #b (fs_tail #c fsG))))
 let helper_var2 g a b c fsG = fs_hd (fs_tail #b (fs_tail #c fsG))
 
+unfold
+val helper_unit : g:env -> fs_oexp g unit (fun _ -> ret ())
+let helper_unit g = fun _ -> ()
+
+unfold
+val helper_true : g:env -> fs_oexp g bool (fun _ -> ret true)
+let helper_true g = fun _ -> true
+
+unfold
+val helper_false : g:env -> fs_oexp g bool (fun _ -> ret false)
+let helper_false g = fun _ -> false
+
+unfold
+val helper_app: #g :env ->
+                #a :Type ->
+                #b :Type ->
+                wpF : spec_env g (a -> b) ->
+                f :fs_oexp g (a -> b) wpF ->
+                wpX : spec_env g a ->
+                x :fs_oexp g a wpX ->
+                fs_oexp g b
+                  (fun fsG ->
+                    pure_bind_wp (a -> b) b (wpF fsG) (fun f' ->
+                      pure_bind_wp a b (wpX fsG) (fun x' ->
+                       ret (f' x'))))
+let helper_app _ f _ x =
+  fun fsG ->
+    M.elim_pure_wp_monotonicity_forall ();
+    (f fsG) (x fsG)
+
+unfold
+val helper_if : #g :env ->
+                #a :Type ->
+                wpC : spec_env g bool ->
+                c   : fs_oexp g bool wpC ->
+                wpT : spec_env g a ->
+                t   : fs_oexp g a wpT ->
+                wpE : spec_env g a ->
+                e   : fs_oexp g a wpE ->
+                fs_oexp g a
+                  (fun fsG ->
+                    pure_bind_wp bool a (wpC fsG) (fun r ->
+                      pure_if_then_else _ r (wpT fsG) (wpE fsG)))
+let helper_if _ c _ t _ e =
+  fun fsG ->
+    M.elim_pure_wp_monotonicity_forall ();
+    if c fsG then t fsG else e fsG
+
+unfold
+val wp_lambda : #g :env ->
+                #a :Type ->
+                #b :Type ->
+                wpBody:spec_env (extend a g) b ->
+                spec_env g (a -> b)
+
+let wp_lambda #g #a #b wpBody fsG : pure_wp (a -> b) =
+  reveal_opaque (`%pure_wp_monotonic) (pure_wp_monotonic);
+  fun (p:pure_post (a -> b)) ->
+    forall (f:a -> b).
+      (forall (p':pure_post b) (fsG':fs_env (extend a g)).
+        fsG == fs_tail fsG' ==>  wpBody fsG' p' ==>  p' (f (fs_hd fsG'))
+      ) ==>  p f
+
+unfold
+val helper_lambda : #g :env ->
+                #a :Type ->
+                #b :Type ->
+                wpBody:spec_env (extend a g) b ->
+                f :fs_oexp g (a -> b) (wp_lambda wpBody) ->
+                fs_oexp (extend a g) b wpBody
+let helper_lambda #g #a _ f =
+  fun fsG -> f (fs_tail #a fsG) (fs_hd fsG)
+
+unfold
+val helper_refv: #g:env ->
+                #a:Type ->
+                #ref1:(a -> Type0) ->
+                ref2:(a -> Type0) ->
+                wpV:spec_env g (x:a{ref1 x}) ->
+                v:fs_oexp g (x:a{ref1 x}) wpV ->
+                fs_oexp g (x:a{ref2 x}) (fun fsG -> refv_wp ref1 ref2 (wpV fsG))
+let helper_refv _ wpV v =
+  fun fsG -> M.elim_pure_wp_monotonicity (wpV fsG);
+    v fsG
+
+unfold
+val helper_seq :#g:env ->
+                #ref1:Type0 ->
+                wpV:spec_env g (_:unit{ref1}) ->
+                v:fs_oexp g (_:unit{ref1}) wpV ->
+                #a:Type ->
+                wpK:spec_env g a ->
+                k:fs_oexp g a wpK ->
+                fs_oexp g a
+                  (fun fsG -> pure_bind_wp (x:unit{ref1}) a (wpV fsG) (fun _ -> wpK fsG))
+let helper_seq _ v _ k =
+  fun fsG -> M.elim_pure_wp_monotonicity_forall ();
+    v fsG ; k fsG
+
 [@@no_auto_projectors] // FStarLang/FStar#3986
 noeq
 type compilable : #a:Type -> g:env -> wp:spec_env g a -> fs_oexp g a wp -> Type =
-| CUnit       : #g:env ->
-                compilable g
-                  (fun _ -> ret ())
-                  (fun _ -> ())
-| CTrue       : #g:env ->
-                compilable g
-                  (fun _ -> ret true)
-                  (fun _ -> true)
-| CFalse      : #g:env ->
-                compilable g
-                  (fun _ -> ret false)
-                  (fun _ -> false)
+| CUnit       : #g:env ->  compilable g _ (helper_unit g)
+| CTrue       : #g:env ->  compilable g _ (helper_true g)
+| CFalse      : #g:env ->  compilable g _ (helper_false g)
 
 | CVar0       : #g:env ->
                 #a:Type ->
                 compilable #a _ _ (helper_var0 g a)
+
 | CVar1       : #g:env ->
                 #a:Type ->
                 #b:Type ->
@@ -114,13 +190,7 @@ type compilable : #a:Type -> g:env -> wp:spec_env g a -> fs_oexp g a wp -> Type 
                 #wpX : spec_env g a ->
                 #x :fs_oexp g a wpX ->
                 cx:compilable g wpX x ->
-                compilable #b g
-                  (fun fsG ->
-                    pure_bind_wp (a -> b) b (wpF fsG) (fun f' ->
-                      pure_bind_wp a b (wpX fsG) (fun x' ->
-                       ret (f' x'))))
-                  (fun fsG -> M.elim_pure_wp_monotonicity_forall ();
-                    (f fsG) (x fsG))
+                compilable #b g _ (helper_app wpF f wpX x)
 
 | CIf         : #g :env ->
                 #a :Type ->
@@ -133,13 +203,7 @@ type compilable : #a:Type -> g:env -> wp:spec_env g a -> fs_oexp g a wp -> Type 
                 #wpE : spec_env g a ->
                 #e   : fs_oexp g a wpE ->
                 ce   : compilable g wpE e ->
-                compilable g
-                  (fun fsG ->
-                    pure_bind_wp bool a (wpC fsG) (fun r ->
-                      pure_if_then_else _ r (wpT fsG) (wpE fsG)))
-                  (fun fsG ->
-                    M.elim_pure_wp_monotonicity_forall ();
-                    if c fsG then t fsG else e fsG)
+                compilable g _ (helper_if wpC c wpT t wpE e)
 
 | CLambda     : #g :env ->
                 #a :Type ->
@@ -158,10 +222,8 @@ type compilable : #a:Type -> g:env -> wp:spec_env g a -> fs_oexp g a wp -> Type 
                 #wpV:spec_env g (x:a{ref1 x}) ->
                 #v:fs_oexp g (x:a{ref1 x}) wpV ->
                 compilable #(x:a{ref1 x}) g wpV v ->
-                compilable #(x:a{ref2 x}) g
-                  (fun fsG -> refv_wp ref1 ref2 (wpV fsG))
-                  (fun fsG -> M.elim_pure_wp_monotonicity (wpV fsG);
-                    v fsG)
+                compilable #(x:a{ref2 x}) g _ (helper_refv ref2 wpV v)
+
 | CSeq        : #g:env ->
                 ref1:Type0 ->
                 #wpV:spec_env g (_:unit{ref1}) ->
@@ -174,10 +236,7 @@ type compilable : #a:Type -> g:env -> wp:spec_env g a -> fs_oexp g a wp -> Type 
                 #wpK:spec_env g a ->
                 #k:fs_oexp g a wpK ->
                 compilable #a g wpK k ->
-                compilable #a g
-                  (fun fsG -> pure_bind_wp (x:unit{ref1}) a (wpV fsG) (fun _ -> wpK fsG))
-                  (fun fsG -> M.elim_pure_wp_monotonicity_forall ();
-                    v fsG ; k fsG)
+                compilable #a g _ (helper_seq wpV v wpK k)
 
 type compilable_closed #a #wp (x:a{forall fsG. wp fsG <= ret x}) =
   compilable empty wp (fun _ -> x)
@@ -185,19 +244,25 @@ type compilable_closed #a #wp (x:a{forall fsG. wp fsG <= ret x}) =
 type compilable_debug #a wp (x:a) (_:squash (forall fsG. wp fsG <= ret x)) =
   compilable_closed #a #wp x
 
+#set-options "--timing"
+
 let test2_var
   : compilable (extend unit (extend unit empty)) _ (fun fsG -> fs_hd (fs_tail fsG))
   = CVar1
 
 let test_app0 ()
-  : (compilable (extend (unit -> unit) empty) _ (fun fsG -> fs_hd fsG ()))
+  : Tot (compilable (extend (unit -> unit) empty) _ (fun fsG -> fs_hd fsG ()))
   = CApp CVar0 CUnit
 
-[@expect_failure] // FIXME
+// FIXME, why does it need tactics to do such simple proofs?
 let test_app1 ()
-  : Tot (compilable (extend (unit -> unit -> unit) empty) _ (fun fsG -> fs_hd fsG () ()))
- // by (explode (); dump "H")
-  = CApp (CApp CVar0 CUnit) CUnit
+  : Tot (compilable (extend (bool -> bool -> bool) empty) _ (fun fsG -> ((fs_hd fsG) true) false))
+  by (explode ();
+      rewrite_eqs_from_context (); assumption ();
+      trefl ();
+      trefl ();
+      trefl ())
+  = CApp (CApp CVar0 CTrue) CFalse
 
 let test1_exp
   : compilable_closed #(unit -> unit) (fun x -> x)
@@ -207,7 +272,6 @@ let test_fapp1 ()
   : Tot (compilable_debug #((unit -> unit) -> unit) _ (fun f -> f ()) ())
   = CLambda (CApp CVar0 CUnit)
 
-[@expect_failure] // FIXME, depends on test_app1
 let test_fapp2
   : compilable_closed #((unit -> unit -> unit) -> unit) (fun f -> f () ())
   = CLambda (CApp (CApp CVar0 CUnit) CUnit)
@@ -272,8 +336,8 @@ let test_always_false'
   : compilable_closed test_always_false
   = CLambda (CRefinement _ (CIf CVar0 (CFalse) CVar0))
 
-let test_always_false''
-  : compilable_closed test_always_false
+let test_always_false'' ()
+  : Tot (compilable_closed test_always_false)
   = CLambda (CIf CVar0 (CRefinement _ CFalse) (CRefinement _ CVar0))
 
 let test_always_false_complex'
@@ -302,20 +366,20 @@ let test_seq_qref'
 
 
 let test_seq_p_implies_q'
-  : compilable_debug _ test_seq_p_implies_q _
+  : compilable_closed test_seq_p_implies_q
   = CLambda (CLambda (CSeq _ (CApp CVar1 CVar0) (CRefinement _ CVar0)))
 
-let test_if_seq'
-  : compilable_debug _ test_if_seq _
+let test_if_seq' ()
+  : Tot (compilable_closed test_if_seq)
   = CLambda (CLambda (
      CIf CVar0
          (CSeq _ (CApp CVar1 (CRefinement _ CVar0))
                      (CRefinement _ CVar0))
          (CRefinement _ CVar0)))
 
-[@expect_failure] // FIXME, depends on test_app1
-let test_context'
-  : compilable_closed test_context
+[@expect_failure]
+let test_context' ()
+  : Tot (compilable_debug _ test_context _)
   = CLambda (CLambda (CIf CVar1
                           (CApp CVar0 (CRefinement (fun _ -> True) #(fun x -> x == true) CVar1))
                           (CLambda #_ #_ #_ #_ #(fun fsG y -> y) CVar0)))
